nola/bi/internal.v
@@ -1,0 +1,45 @@
+(** * On internal equality *)
+
+From nola Require Export prelude.
+From iris.bi Require Export bi.
+From iris.proofmode Require Import proofmode.
+
+Implicit Type PROP : bi.
+
+(** ** Lemmas on [internal_eq] *)
+Section internal_ne.
+  Context `{!BiInternalEq PROP}.
+
+  (** Variants of [f_equivI] *)
+  Lemma f_equivI_exist {A PROP'} {Φ Ψ : A → PROP'} :
+    (∀ a, Φ a ≡ Ψ a) ⊢@{PROP} (∃ a, Φ a) ≡ (∃ a, Ψ a).
+  Proof. rewrite -discrete_fun_equivI. apply f_equivI. solve_proper. Qed.
+  Lemma f_equivI_forall {A PROP'} {Φ Ψ : A → PROP'} :
+    (∀ a, Φ a ≡ Ψ a) ⊢@{PROP} (∀ a, Φ a) ≡ (∀ a, Ψ a).
+  Proof. rewrite -discrete_fun_equivI. apply f_equivI. solve_proper. Qed.
+End internal_ne.
+
+(** ** [internal_ne] Non-expansiveness inside [PROP] *)
+Section internal_ne.
+  Context `{!BiInternalEq PROP, !BiPlainly PROP}.
+  Implicit Type A B : ofe.
+
+  Definition internal_ne {A B} (f : A -d> B) : PROP :=
+    ∀ a a', a ≡ a' → f a ≡ f a'.
+  (** [internal_ne] is non-expansive *)
+  #[export] Instance internal_ne_ne {A B} : NonExpansive (@internal_ne A B).
+  Proof. solve_proper. Qed.
+  #[export] Instance internal_ne_proper {A B} :
+    Proper ((≡) ==> (≡)) (@internal_ne A B).
+  Proof. solve_proper. Qed.
+  (** [internal_ne] is plain *)
+  #[export] Instance internal_ne_plain {A B f} : Plain (@internal_ne A B f).
+  Proof. exact _. Qed.
+  #[export] Instance internal_ne_persistent {A B f} :
+    Persistent (@internal_ne A B f).
+  Proof. exact _. Qed.
+  (** [NonExpansive] entails [internal_ne] *)
+  Lemma ne_internal_ne {A B} `{!NonExpansive f} : ⊢ @internal_ne A B f.
+  Proof. iIntros (??) "≡". by iRewrite "≡". Qed.
+End internal_ne.
+Arguments internal_ne : simpl never.
