README.md
@@ -73,6 +73,7 @@ All the Coq code is in [`nola/`](nola/) and structured as follows:
     [`cit`](nola/util/cit.v) (Coinductive-inductive tree)
 - [`bi/`](nola/bi/) : Libraries for bunched implication logic
   + [`util`](nola/bi/util.v) (Utilities)
+  + [`internal`](nola/bi/internal.v) (Internal equality)
   + [`gmap`](nola/bi/gmap.v) (On `gmap`),
     [`plist`](nola/bi/plist.v) (On `plist`)
   + [`order`](nola/bi/order.v) (Order theory),
